% chktex-file 3 chktex-file 18 chktex-file 36

\section*{Exercise 5.}

What can be concluded from the previous exercise if
\begin{enumerate}[label = (\alph*)]
    \item The pole of $f$ is not at 1 but at $e^{i\phi}$ for some $\phi \in \R$.
    \item The pole is of order $k \geq 1$.
\end{enumerate}

\textbf{Solution (a):}

Let $\zeta \in \{z\in\C \;:\; |z| = 1\}$ be the simple pole of $f$ in $U$. Then, for $\lambda \neq 0$
\[ f(z) = \frac{\lambda}{\zeta-z} + h(z) = \frac{\lambda}{\zeta(1-z/\zeta)} + h(z), \]
where, again, $h$ is holomorphic at $U$ and has a Taylor series $h(z) = \sum_{k = 0}^{\infty} b_k z^k$ with radius of convergence strictly greater than one, and thus, $b_n \to 0$ as $n\to \infty$. Also, when $|z| < 1$,
\[ \frac{\lambda}{\zeta(1-z/\zeta)} = \frac{\lambda}{\zeta} \sum_{k = 0}^{\infty} \zeta^{-k} z^k = \lambda\sum_{k = 0}^{\infty} \zeta^{-k-1} z^k . \]
Put everything together to obtain:
\[ f(z) = \sum_{n = 0}^{\infty} a_n z^n = \sum_{n = 0}^{\infty} (b_n - \lambda \zeta^{-n-1}) z^n. \]
By uniqueness of the power series expansion
\[ a_n = b_n - \lambda \zeta^{-n-1}. \]
Also note that $|b_n \zeta^{n}| = |b_n| \to 0$ so it follows that
\[ \lim_{n\to\infty} \frac{a_{n+1}}{a_n} = \lim_{n\to\infty} \frac{b_{n+1} - \lambda \zeta^{-n-2}}{b_n - \lambda \zeta^{-n-1}} = \frac{b_{n+1} \zeta^{n+2} - \lambda}{b_n\zeta^{n+2} - \lambda \zeta^{-1} } = \frac{ - \lambda}{ - \lambda \zeta^{-1} } = \zeta.\]

\textbf{Solution (b):}

If there's a pole of order 2 at $\zeta$, then, there exists $\lambda_1, \lambda_2 \neq 0$ such that
\[ f(z) = \frac{\lambda_2}{\zeta^2 (1-z/\zeta)^2} + \frac{\lambda_1}{\zeta(1-z/\zeta)} + h(z), \]
where, $h(z) = \sum_{n = 0}^{\infty} b_n z^n$ has the same properties we mentioned before ($b_n \zeta^n \overset{n \to \infty}{\to} 0$). Note that
\[ \frac{d}{dz} \frac{1}{1-z/\zeta} = \frac{1}{(1-z/\zeta)^2}, \]
so the power series expansion of $\frac{1}{(1-z/\zeta)^2}$ when $|z| < 1$ is
\[ \frac{1}{(1-z/\zeta)^2} = \sum_{n = 0}^{\infty} \zeta^{-n} \frac{d z^n}{dz}  = \sum_{n = 0}^{\infty} n \zeta^{-n} z^{n-1} =  \sum_{n = 0}^{\infty} (n+1) \zeta^{-n-1} z^{n}.\]
It follows that
\[ \everymath{\displaystyle}
\arraycolsep=1.8pt\def\arraystretch{2.5}
\begin{array}{rcl}
    f(z) & = & \sum_{n = 0}^{\infty} a_n z^n \\
    & = & \frac{\lambda_2}{\zeta^2} \sum_{n = 0}^{\infty} \zeta^{-n-1} (n+1) z^{n} + \frac{\lambda_1}{\zeta}\sum_{n = 0}^{\infty} \zeta^{-n} z^{n} + \sum_{k = 0}^{\infty}b_n z^{n}\\
    & = & \sum_{n = 0}^{\infty} \lambda_2 \zeta^{-n-3} (n+1) z^{n} + \sum_{n = 0}^{\infty} \lambda_1 \zeta^{-n-1} z^{n} + \sum_{k = 0}^{\infty}b_n z^{n}
\end{array} \]
\[ \implies a_n = \lambda_2 \zeta^{n-3} (n+1) + \lambda_1 \zeta^{n-1} + b_n \]
Then,
\[ \everymath{\displaystyle}
\arraycolsep=1.8pt\def\arraystretch{2.5}
\begin{array}{rcl}
    \lim_{n\to\infty} \frac{a_{n+1}}{a_n} 
    & = & \lim_{n\to\infty} \frac{\lambda_2 \zeta^{-n-4} (n+2)+ \lambda_1 \zeta^{-n-2} + b_{n+1}}{\lambda_2 \zeta^{-n-3} (n+1)+ \lambda_1 \zeta^{-n-1} + b_n}\\
    & = & \lim_{n\to\infty} \frac{\lambda_2 \zeta (n+2)}{\lambda_2 (n+1)}\\
    & = & \zeta.
\end{array} \]

Now, for any $k \geq 1$, note that when $|z| < 1$
\[ \everymath{\displaystyle}
\arraycolsep=1.8pt\def\arraystretch{2.5}
\begin{array}{rcl}
    \frac{\lambda_k}{\zeta^{k}} \cdot \frac{1}{(1-z/\zeta)^k} 
    & = & \frac{\lambda_k}{\zeta^{k}} \cdot \frac{1}{(k-1)!} \cdot \frac{d^{k-1}}{dz^{k-1}} \frac{1}{1-z}\\
    & = & \frac{\lambda_k}{\zeta^{k}(k-1)!} \sum_{n = 0}^{\infty} \underbrace{(n+k-1)\cdots (n+1)}_{= (n+k-1)!/n!} z^{n} \zeta^{-n-k+1}\\
    & = & \sum_{n = 0}^{\infty} \binom{n+k-1}{n}\lambda_k \zeta^{-n-2k+1} z^n
\end{array}\]

Then, let $K\geq 1$ the order of the pole of $f$ at $\zeta$,
\[ \everymath{\displaystyle}
\arraycolsep=1.8pt\def\arraystretch{2.5}
\begin{array}{rcl}
    f(z) & = & \sum_{k = 1}^{K} \frac{\lambda_k}{(\zeta - z)^k} + h(z)\\
    & = & \sum_{k = 1}^{K}\sum_{n = 0}^{\infty} \binom{n+k-1}{n}\lambda_k \zeta^{-n-2k+1} z^n + \sum_{n = 0}^{\infty} b_n z^n.
\end{array} \]
So it follows that
\[ a_n = b_n + \sum_{k = 1}^{K} \binom{n+k-1}{n}\lambda_k \zeta^{-n-2k+1} \]
Finally, $b_n \to 0$ and $\binom{n+K-1}{n}$ dominates the expression since is the polynomial of $n$ with greatest degree, so it follows that
\[ \everymath{\displaystyle}
\arraycolsep=1.8pt\def\arraystretch{2.5}
\begin{array}{rcl}
    \lim_{n\to\infty} \frac{a_{n+1}}{a_n} & = & \lim_{n\to\infty} \tfrac{b_{n+1} + \sum_{k = 1}^{K} \binom{n+k}{n+1}\lambda_k \zeta^{-n-2k}}{b_n + \sum_{k = 1}^{K} \binom{n+k-1}{n}\lambda_k \zeta^{-n-2k+1}}\\
    & = & \lim_{n\to\infty} \frac{n^{K}\lambda_k \zeta}{n^{K}\lambda_k} = \zeta.
\end{array} \]