% chktex-file 3 chktex-file 18 chktex-file 36
\section*{Exercise 3.}

Determine the Laurent series of $f(z) = \frac{1}{z(z-1)(z-2)}$ in the regions $U_1 := \{0<|z|<1\},\; U_2 := \{1<|z|<2\},\; U_3 := \{|z|>2\}$

\textbf{Solution:}

The partial fraction decomposition is the following
\[ \everymath{\displaystyle}
\arraycolsep=1.8pt\def\arraystretch{2.5}
\begin{array}{rcl}
    f(z) = \frac{1}{z(z-1)(z-2)} & = & \frac{1}{2z} + \frac{1}{1-z} - \frac{1}{2(2-z)}\\
    & = & \frac{1}{2z} + \frac{1}{1-z} - \frac{1}{4}\frac{1}{1-z/2}
\end{array}\]

For $0<|z|<1 $, the functions $1/(1-z)$ and $1/(1-z/2)$ have convergent power series. Therefore, the Laurent series is the following
\[ \everymath{\displaystyle}
\arraycolsep=1.8pt\def\arraystretch{2.5}
\begin{array}{rcl}
    f(z) & = & \frac{1}{2z} + \sum_{k = 0}^{\infty} z^k - \frac{1}{4} \sum_{k = 0}^{\infty} \frac{z^k}{2^k}\\
    & = & \frac{1}{2z} + \sum_{k = 0}^{\infty} z^k \left( 1-\frac{1}{2^{k+2}} \right)\\
    & = & \frac{1}{2z} + \frac{3}{4} + \frac{7z}{8} + \frac{15z^2}{16} + \cdots\\
    & = & \sum_{k = -1}^{\infty} z^k \left( 1-\frac{1}{2^{k+2}}\right)
\end{array} \]

For the case $1<|z|<2$, $1/(1-z/2)$ has a power series expansion but $1/(1-z)$ doesn't. Instead, we use $1/(1-z) = \dfrac{1}{z(1-1/z)}$:
\[ \everymath{\displaystyle}
\arraycolsep=1.8pt\def\arraystretch{2.5}
\begin{array}{rcl}
    f(z) & = & \frac{1}{2z} - \frac{1}{z}\frac{1}{1-1/z} - \frac{1}{4}\frac{1}{1-z/2}\\
    & = & \frac{1}{2z} - \frac{1}{z}\sum_{k = 0}^{\infty} \frac{1}{z^k} - \frac{1}{4} \sum_{k = 0}^{\infty} \frac{z^k}{2^k}\\
    & = & \sum_{k = 2}^{\infty} \frac{-1}{z^k} - \frac{1}{2z} - \sum_{k = 0}^{\infty} \frac{z^k}{2^{k+2}}
\end{array} \]

Finally, for the case $|z|>2$, neither $1/(1-z/2)$ nor $1/(1-z)$ have geometric series expansions, but $1/(1-z) = \dfrac{-1}{z(1-1/z)}$ and $\dfrac{-1}{(z/2)(1-2/z)}$

\[ \everymath{\displaystyle}
\arraycolsep=1.8pt\def\arraystretch{2.5}
\begin{array}{rcl}
    f(z) & = & \frac{1}{2z} - \frac{1}{z}\frac{1}{1-1/z} + \frac{1}{4(z/2)}\frac{1}{1-2/z}\\
    & = & \frac{1}{2z} - \frac{1}{z}\sum_{k = 0}^{\infty} \frac{1}{z^k} + \frac{1}{4(z/2)} \sum_{k = 0}^{\infty} \frac{2^k}{z^k}\\
    & = & \frac{1}{2z} - \sum_{k = 1}^{\infty} \frac{1}{z^{k}} + \sum_{k = 1}^{\infty} \frac{2^{k-2}}{z^{k}}\\
    & = & \frac{1}{z} \left( \frac{1}{2} - 1 +\frac{1}{2} \right) + \sum_{k = 2}^{\infty} \frac{1}{z^{k}} (2^{k-2}-1)\\
    & = & \sum_{k = 2}^{\infty} \frac{1}{z^{k}} (2^{k-2}-1)
\end{array} \]