% chktex-file 3 chktex-file 18 chktex-file 36 chktex-file 40
\section*{Exercise 3.}

\begin{enumerate}[label=(\alph*)]
    \item $\exp(z+w) = \exp(z) \exp(w)$.
    \item $\exp(z) \neq 0$ for all $z\in\C$.
    \item $|\exp(z)| = 1$ if and only if $z\in i\R$.
    \item $\cos^2(z)+\sin^2(z) = 1$ for all $z \in \C$.
    \item $\cos(z+ 2\pi) = \cos(z)$ and $\sin(z+2\pi) = \sin(z)$ for all $z \in \C$.
    \item $\cos(z) = 0$ or $\sin(z) = 0$ $\implies$ $z\in\R$.
    \item For every $x\in\R$, $\lim_{t\to\pm\infty}|\cos(x+it)| = \infty $ and $\lim_{t\to\pm\infty}|\sin(x+it)| = \infty $. The limit is uniform in $x$.
\end{enumerate}

\subsection*{Solution Part (a)}
The Cauchy product of 2 series implies that
\[ \everymath{\displaystyle}
\arraycolsep=1.8pt\def\arraystretch{2.5}
\begin{array}{rcl}
    \exp (z) \exp (w) & = & \left( \sum_{n = 0}^{\infty} \frac{z^n}{n!} \right) \left( \sum_{m = 0}^{\infty} \frac{w^m}{m!} \right)\\
    & = & \sum_{n = 0}^{\infty} \sum_{k = 0}^n \frac{z^k w^{n-k}}{k!(n-k)!}\\
    & = & \sum_{n = 0}^{\infty} \sum_{k = 0}^n \frac{z^k w^{n-k}}{k!(n-k)!} \cdot \frac{n!}{n!}\\
    & = & \sum_{n = 0}^{\infty} \frac{1}{n!} \sum_{k = 0}^n \binom{n}{k} z^k w^{n-k}\\
    & = & \sum_{n = 0}^{\infty} \frac{(z+w)^n}{n!}\\
    & = & \exp(z+w)
\end{array} \]

\subsection*{Solution Part (b)}

For every complex number $z$, there exists an additive inverse $(-z)$ such that
\[ z + (-z) = 0. \]
Thus, if it was the case that there exists $z\in \C$ such that $e^z = 0$. Then, using part (a),
\[ 1 = e^0 = e^{z + (-z)} = e^{z} e^{-z} = 0, \]
and this would lead to a contradiction.

\subsection*{Solution Part (c)}

$\boldsymbol{\impliedby:}$ Let $z = iy,\; y\in \R$. We are going to prove Euler's formula:
\[ \everymath{\displaystyle}
\arraycolsep=1.8pt\def\arraystretch{2.5}
\begin{array}{rcl}
    \exp(iy) & = & \frac{(iy)^0}{0!} + \frac{(iy)^1}{1!} + \frac{(iy)^2}{2!} + \frac{(iy)^3}{3!} + \cdots\\
    & = & \left( \frac{(iy)^0}{0!} + {(iy)^2}{2!} + \cdots \right) + i\left( \frac{y^1}{0!} + {y^3}{2!} + \cdots \right) 
\end{array} \]

$\boldsymbol{\implies:}$ Let $z = x+iy,\; x,y\in\R$ such that $|\exp(z)| = 1$. Then, using part (a), $|\exp(z)| = |\exp(x)| |\exp(iy)|$