% chktex-file 3 chktex-file 9 chktex-file 17 chktex-file 18 chktex-file 36

\section{Exercise 1.}

Determine whether the following products converge:
\[
(\mbox{a})\;\prod_{n=1}^{\infty} \left( 1 + \frac{(-1)^n}{n} \right), \quad (\mbox{b})\;\prod_{n=1}^{\infty} \left( 1 + \frac{(-1)^n}{\sqrt{n}} \right).
\]

\textbf{Note:} The first term in both products is 0, so we are going to skip and show that the tails from $n = 2$ forward converge (or diverge) for both cases.

\subsection*{Solution Item (a)}

We are going to prove that $\sum_{n = 2}^{\infty}\log\left( 1+\frac{(-1)^n}{n} \right)$ converges. In fact, if $M$ is even,
\[ \everymath{\displaystyle}
\arraycolsep=1.8pt\def\arraystretch{2.5}
\begin{array}{rcl}
    \sum_{n = 2}^{M}\log\left( 1+\frac{(-1)^n}{n} \right) & = & 
    \sum_{k = 1}^{M/2}\log\left( \frac{2k+1}{2k}\right) + \log\left(\frac{2k}{2k+1}\right)\\
    & = & \sum_{k = 1}^{M/2} \log\left( \frac{2k+1}{2k}\cdot\frac{2k}{2k+1}\right)\\
    & = & 0,
\end{array} \]
and if $M = 2K+1$ is odd,
\[ \everymath{\displaystyle}
\arraycolsep=1.8pt\def\arraystretch{2.5}
\begin{array}{rcl}
    \sum_{n = 2}^{M}\log\left( 1+\frac{(-1)^n}{n} \right) & = & \log\left(\frac{2K}{2K+1}\right) + 
    \sum_{k = 1}^{(M-1)/2}\log\left( \frac{2k+1}{2k}\right) + \log\left(\frac{2k}{2k+1}\right)\\
    & = & \log\left(\frac{2K}{2K+1}\right).
\end{array} \]
Since $\log$ is continuous at 1 and $\frac{2K}{2K+1} \to 1$ when $K\to \infty$, we conclude that $\log\left(\frac{2K}{2K+1}\right)$ converges to 0. Since the entire log-series converges to 0, it must follow that
\[ \prod_{n=2}^{\infty} \left( 1 + \frac{(-1)^n}{n} \right) = \exp\left[ \sum_{n = 2}^{\infty}\log\left( 1+\frac{(-1)^n}{n} \right)  \right] = 1. \]

\subsection*{Solution Item (b)}

Now, we are going to prove that $\sum_{n = 2}^{\infty}\log\left( 1+\frac{(-1)^n}{\sqrt{n}} \right)$ diverges. In fact, we are going to show that the subsequence $\sum_{n = 1}^M\log\left( 1+\frac{(-1)^n}{\sqrt{n}} \right)$ with $M = 2k$ diverges to $-\infty$. Note that
\[ \everymath{\displaystyle}
\arraycolsep=1.8pt\def\arraystretch{2.5}
\begin{array}{rcl}
    \log\left( 1+\frac{1}{\sqrt{2n}} \right) +  \log\left( 1-\frac{1}{\sqrt{2n+1}} \right) & = & \log \left[ \left( 1+\frac{1}{\sqrt{2n}} \right) \cdot \left( 1-\frac{1}{\sqrt{2n+1}} \right) \right]\\
    & = & \log\left[1 + \frac{\sqrt{2n+1}-\sqrt{2n}-1}{\sqrt{2n} \cdot \sqrt{2n+1}} \right]
\end{array} \]

By the limit comparison test $\log(1+x) = x - O(x^{2}) \approx x$ for $x$ near to 0. Then, we can compare the series of $ a_n = \log\left[1 + \frac{\sqrt{2n+1}-\sqrt{2n}-1}{\sqrt{2n} \cdot \sqrt{2n+1}} \right]$ with the series of $b_n = \frac{\sqrt{2n+1}-\sqrt{2n}-1}{\sqrt{2n} \cdot \sqrt{2n+1}}$. 

\textbf{Remark:} Note that for $n \geq 1$, $\sqrt{2n+1}-\sqrt{2n}-1 < 0 $. The limit comparison test only applies if $a_n, b_n > 0$, but for our case,
\[ a_n = \log\left[1 + \frac{\sqrt{2n+1}-\sqrt{2n}-1}{\sqrt{2n} \cdot \sqrt{2n+1}} \right] < 0 \mbox{ and } b_n = \frac{\sqrt{2n+1}-\sqrt{2n}-1}{\sqrt{2n} \cdot \sqrt{2n+1}} < 0 \]
and thus, the same argument can be applied to $-a_n, -b_n > 0$ to conclude that $-\sum_n a_n$ diverges because $-\sum_n b_n$ does.

Since $a_n = \log(1+b_n)$ and $b_n \to 0$ when $n\to \infty$, by uniqueness of limit and then L-h√¥spital rule,
\[ \lim_{n\to\infty} \frac{a_n}{b_n} = \lim_{x\to 0} \frac{\log(1+x)}{x} = \lim_{x\to 0} \frac{1}{1+x} = 1. \]
Then, we can also compare $b_n$ with $c_n = \frac{-1}{2n}$ because
\[ \everymath{\displaystyle}
\arraycolsep=1.8pt\def\arraystretch{2.5}
\begin{array}{rcl}
    \frac{b_n}{c_n} & = & \frac{\sqrt{2n+1}-\sqrt{2n}-1}{\sqrt{2n} \cdot \sqrt{2n+1}} \cdot (-2n) \\
    & = & \underbrace{\sqrt{\frac{2n}{2n+1}}}_{\to 1} + \underbrace{\frac{2n}{\sqrt{2n+1}} - \sqrt{2n}}_{\to 0}\\
    & \to & 1,\quad n\to \infty
\end{array} \]

Finally, since $\sum_{n = 1}^{\infty} c_n = \sum_{n = 1}^{\infty} \frac{-1}{2n} $ diverges to $-\infty$, it follows that $\sum_{n = 1}^{\infty} b_n$ diverges, and thus, $\sum_{n = 1}^{\infty} a_n$ diverges to $-\infty$ too. Therefore,
\[ \everymath{\displaystyle}
\arraycolsep=1.8pt\def\arraystretch{2.5}
\begin{array}{rcl}
    \sum_{n = 2}^{2k}\log\left( 1+\frac{(-1)^n}{\sqrt{n}} \right) & = & \sum_{n = 1}^{k} \log\left[1 + \frac{\sqrt{2n+1}-\sqrt{2n}-1}{\sqrt{2n} \cdot \sqrt{2n+1}} \right]\\
     & = & \sum_{n = 1}^{k} a_n \to -\infty,\quad M \to \infty.
\end{array}  \]
That implies that $\prod_{n = 2}^{\infty} \left( 1+\frac{(-1)^n}{\sqrt{n}} \right)$ has a subsequence that diverges to 0.