% chktex-file 3 chktex-file 18 chktex-file 36
\section*{Exercise 1.}

Calculate the principal part at 0 of the functions
\[ f(z) = \frac{(\sin z)^2}{\sin(z^2)}, \hspace{2em} g(z) = \frac{1-z^2}{z(1-\cos(z^2))}.  \]

\subsection*{Solution Item (a)}
The Taylor series of $(\sin z)^2$ is by trigonometric identities,
\[ \everymath{\displaystyle}
\arraycolsep=1.8pt\def\arraystretch{2.5}
\begin{array}{rcl}
    (\sin z)^2 & = & \frac{1-\cos(2z)}{2}\\
    & = & \frac{1}{2} - \sum_{n = 0}^{\infty} \frac{(-1)^n 2^{2n-1}}{(2n)!} z^{2n}\\
    & = & z^2 - \frac{2^3 z^4}{4!} + \frac{2^5 z^6}{6!} + O(z^8)
\end{array} \]

The Taylor series of $\sin (z^2)$ is by substitution
\[ \everymath{\displaystyle}
\arraycolsep=1.8pt\def\arraystretch{2.5}
\begin{array}{rcl}
    \sin(z^2) & = & \sum_{n = 0}^{\infty} \frac{(-1)^n z^{4n+1}}{(2n+1)!}\\
    & = & z^2 - \frac{z^6}{3!} + \frac{z^{10}}{5!} + O(z^{14})
\end{array} \]

Then,
\[ \everymath{\displaystyle}
\arraycolsep=1.8pt\def\arraystretch{2.5}
\begin{array}{rcl}
    \lim_{z\to 0} \frac{(\sin z)^2}{\sin(z^2)} & = & \lim_{z\to 0} \frac{z^2 - \frac{2^3}{4!} z^4 + O(z^6) }{z^2 + O(z^6)}\\
    & = & \lim_{z\to 0} \frac{1 + O(z^2)}{1 + O(z^4)} = 1.
\end{array} \]

Therefore, the principal part of the series is 0 because the series has a removable singularity at 0.

\subsection*{Solution Item (b)}

The Taylor series expansion of $z(1-\cos(z^2))$ is the following
\[ \everymath{\displaystyle}
\arraycolsep=1.8pt\def\arraystretch{2.5}
\begin{array}{rcl}
    z(1-\cos(z^2)) & = & z \left( 1 - \sum_{n = 0}^{\infty} \frac{(-1)^n}{(2n)!} z^{2n} \right)\\
    & = & \sum_{n = 1}^{\infty} \frac{(-1)^{n+1}}{(2n)!} z^{2n+1}\\
    & = & \frac{1}{2!} z^5 - \frac{1}{4!} z^9 + O(z^{13})
\end{array} \]
Therefore,
\[ g(z) = \frac{1 - z^2}{\frac{1}{2} z^5 + O(z^9)}, \]
so it's clear that $g(z)$ has a pole of order 5 at $z = 0$. In fact, if
\[ g(z) = \sum_{n = -5}^{\infty} a_{n} z^n, \]
then $a_{-5} = \lim_{z\to 0} z^5 g(z) = \lim_{z\to 0} \frac{1- z^2}{\frac{1}{2} + O(z^4)} = 2$. Then, for the next coefficients
\[ \everymath{\displaystyle}
\arraycolsep=1.8pt\def\arraystretch{2.5}
\begin{array}{rcl}
    a_{-4} & = & \lim_{z\to 0} z^4 (g(z) - a_{-5} z^{-5}) \\
    & = & \lim_{z\to 0} z^4 (g(z) - 2z^{-5})\\
    & = & \lim_{z\to 0} z^4 \frac{1-z^2 - 2z^{-5}(\frac{1}{2!} z^5 + O(z^9))}{\frac{1}{2} z^5 + O(z^9)}\\
    & = & \lim_{z\to 0} \frac{-z^2 + O(z^4)}{\frac{1}{2} z + O(z^5)} = 0
\end{array} \]

\[ \everymath{\displaystyle}
\arraycolsep=1.8pt\def\arraystretch{2.5}
\begin{array}{rcl}
    a_{-3} & = & \lim_{z\to 0} z^3 (g(z) - a_{-5} z^{-5} - a_{-4} z^{-4}) \\
    & = & \lim_{z\to 0} z^3 (g(z) - 2z^{-5})\\
    & = & \lim_{z\to 0} z^3 \frac{1-z^2 - 2z^{-5}(\frac{1}{2!} z^5 + O(z^9))}{\frac{1}{2} z^5 + O(z^9)}\\
    & = & \lim_{z\to 0} \frac{-z^2 + O(z^4)}{\frac{1}{2} z^2 + O(z^4)} = -2
\end{array} \]

\[ \everymath{\displaystyle}
\arraycolsep=1.8pt\def\arraystretch{2.5}
\begin{array}{rcl}
    a_{-2} & = & \lim_{z\to 0} z^2 (g(z) - a_{-5} z^{-5} - a_{-4} z^{-4} - a_{-3} z^{-3}) \\
    & = & \lim_{z\to 0} z^2 (g(z) - 2z^{-5} + 2z^{-3})\\
    & = & \lim_{z\to 0} z^2 \frac{1-z^2 + (- 2z^{-5} + 2z^{-3})(\frac{1}{2!} z^5 - \frac{1}{4!} z^9 + O(z^{13}))}{\frac{1}{2} z^5 + O(z^9)}\\
    & = & \lim_{z\to 0} \frac{1 - z^2 + (-1 + \frac{2}{4!} z^{4} + O(z^8)) + (z^2 - \frac{2}{4!} z^{6} + O(z^{10}))}{\frac{1}{2} z^3 + O(z^7)}\\
    & = & \lim_{z\to 0} \frac{\frac{1}{12} z^{4} + O(z^6) }{\frac{1}{2}z^3 + O(z^7)} = 0.
\end{array} \]

\[ \everymath{\displaystyle}
\arraycolsep=1.8pt\def\arraystretch{2.5}
\begin{array}{rcl}
    a_{-1} & = & \lim_{z\to 0} z (g(z) - a_{-5} z^{-5} - a_{-4} z^{-4} - a_{-3} z^{-3} - a_{-2} z^{-2}) \\
    & = & \lim_{z\to 0} z (g(z) - 2z^{-5} + 2z^{-3})\\
    & = & \lim_{z\to 0} z \frac{1-z^2 + (- 2z^{-5} + 2z^{-3})(\frac{1}{2!} z^5 - \frac{1}{4!} z^9 + O(z^{13}))}{\frac{1}{2} z^5 + O(z^9)}\\
    & = & \lim_{z\to 0} \frac{1 - z^2 + (-1 + \frac{2}{4!} z^{4} + O(z^8)) + (z^2 - \frac{2}{4!} z^{6} + O(z^{10}))}{\frac{1}{2} z^4 + O(z^8)}\\
    & = & \lim_{z\to 0} \frac{\frac{1}{12} z^{4} + O(z^6) }{\frac{1}{2}z^4 + O(z^8)} = \frac{1}{6}.
\end{array} \]

Finally, the principal part is
\[ \frac{2}{z^5} - \frac{2}{z^3} + \frac{1}{6z}. \]